# EXERCISE 2-SOLUTIONS 

SGN-1156 Signal Processing Techniques<br>http://www.cs.tut.fi/courses/SGN-1156<br>Tampere University of Technology<br>Germán Gómez-Herrero, http://germangh.com

December 4, 2009

Important: The most important information of Chapter 3 of the book is in tables 3.1, 3.2 and specially 3.3 and 3.4. When computing DTFTs it is often useful to know that:

$$
\sum_{n=m}^{k} r^{n}=\frac{r^{k+1}-r^{m}}{r-1}
$$

Note that I made a mistake when writing the expression above in the whiteboard. Thanks to Junsheng for reporting this. Other useful sums are:

$$
\begin{aligned}
\sum_{n=0}^{\infty} r^{n}=\frac{1}{1-r} & |r|<1 \\
\sum_{n=0}^{\infty} n r^{n} & =\frac{r}{(1-r)^{2}}
\end{aligned}
$$

Remember also the relationships:

$$
\begin{aligned}
& \cos \omega=\frac{e^{j \omega}+e^{-j \omega}}{2} \\
& \sin \omega=\frac{e^{j \omega}-e^{-j \omega}}{2 j}
\end{aligned}
$$

PROBLEM 1: Determine the DTFT of each of the following sequences:
(a) $x_{a}[n]=\mu[n]-\mu[n-5]$
(b) $x_{b}[n]=\alpha^{n}(\mu[n]-\mu[n-8]) \quad|\alpha|<1$
(c) $x_{c}[n]=(n+1) \alpha^{n} \mu[n] \quad|\alpha|<1$

SOLUTION: There are two ways of computing the DTFT of a sequence. Either you apply directly the formula of the DTFT or you try to express your sequence as a linear combination of elementary sequences for which you know the DTFT.
(a)

Using directly the DTFT formula:

$$
X_{a}\left(e^{j \omega}\right)=\sum_{n=0}^{\infty} x_{a}[n] e^{-j \omega n}=\sum_{n=0}^{4} e^{j \omega n}=\frac{e^{-j \omega 5}-1}{e^{-j \omega}-1}
$$

Using the fact that the DTFT of the unit step function is:

$$
\mu[n] \xrightarrow{D T F T} G\left(e^{j \omega}\right)=\frac{1}{1-e^{-j \omega}}+\sum_{k=-\infty}^{\infty} \pi \delta(\omega+2 \pi k)
$$

then:

$$
X_{a}\left(e^{j \omega}\right)=G\left(e^{j \omega}\right)-e^{-j \omega 5} G\left(e^{j \omega}\right)=\frac{1-e^{-j \omega 5}}{1-e^{-j \omega}}-\underbrace{\left(1-e^{-j \omega 5}\right) \sum_{k=-\infty}^{\infty} \pi \delta(\omega+2 \pi k)}_{=0 \forall \omega}
$$

So we finally obtain:

$$
X_{a}\left(e^{j \omega}\right)=\frac{1-e^{-j \omega 5}}{1-e^{-j \omega}}
$$

(b)

$$
X_{b}\left(e^{j \omega}\right)=\frac{1-\alpha^{8} e^{-j \omega 8}}{1-\alpha e^{-j \omega}}
$$

(c)

$$
X_{c}\left(e^{j \omega}\right)=\frac{1}{\left(1-\alpha e^{-j \omega}\right)^{2}}
$$

PROBLEM 2: (problem 3.41 from the book) Let $G_{1}\left(e^{j \omega}\right)$ denote the discretetime Fourier transform of the sequence $g_{1}[n]$ shown in the figure below. Express the DTFTs of $g_{2}[n], g_{3}[n]$ and $g_{4}[n]$ in terms of $G_{1}\left(e^{j \omega}\right)$. Do not evaluate $G_{1}\left(e^{j \omega}\right)$.


## SOLUTION:

$g_{2}[n]=g_{1}[n]+g_{1}[n-4] \Rightarrow G_{2} e^{j \omega}=\left(1+e^{-4 j \omega}\right) G_{1}\left(e^{j \omega}\right)$
$g_{3}[n]=g_{1}[-(n-3)]+g_{1}[n-4] \Rightarrow G_{3} e^{j \omega}=e^{-j 3 \omega} G_{1}\left(e^{-j \omega}\right)+e^{-j 4 \omega} G_{1}\left(e^{j \omega}\right)$
$g_{4}[n]=g_{1}[n]+g_{1}[-(n-7)] \Rightarrow G_{4}\left(e^{j \omega}\right)=G_{1}\left(e^{j \omega}\right)+e^{-j 7 \omega} G_{1}\left(e^{-j \omega}\right)$

PROBLEM 3: Consider the following interconnection of linear shift-invariant systems:


Express the frequency response of the overall system $H\left(e^{j \omega}\right)$ in terms of the frequency responses of the subsystems $H_{1}\left(e^{j \omega}\right), H_{2}\left(e^{j \omega}\right)$, and $H_{3}\left(e^{j \omega}\right)$.

## SOLUTION:

The first step is to represent the given system in frequency domain and to introduce new intermidiate variables in any interconnection between diagram elements. This is shown below:


For simplicity we have omitted all the terms $\left(e^{j \omega}\right)$ in the diagram above. Unless otherwise stated uppercase letters will denote Fourier-domain variables and lower-case letters time-domain ones. We can now write all the system equations in Fourier domain:

$$
\begin{align*}
Y & =A-B  \tag{1}\\
A & =D+C  \tag{2}\\
B & =H_{2} \cdot C  \tag{3}\\
C & =H_{3} \cdot Y  \tag{4}\\
D & =H_{1} \cdot X \tag{5}
\end{align*}
$$

The overall frequency response is defined as $H=\frac{Y}{X}$. Therefore, we need to combine the five equations above into a single one that has only $X$ and $Y$ as unknowns. Combining Eqs. 1, 2 and 3 we obtain:

$$
\begin{equation*}
Y=D+\left(1-H_{2}\right) C \tag{6}
\end{equation*}
$$

Now combining Eq. 6 with Eqs. 4 and 5 we get to:

$$
\begin{equation*}
Y=H_{1} \cdot X+\left(1-H_{2}\right) H_{3} Y \tag{7}
\end{equation*}
$$

which has only two unknowns: $X$ and $Y$. Reorganizing Eq. 7 we finally obtain the overall frequency response of the system:

$$
\begin{equation*}
Y=\frac{H_{1}}{1+H_{3}\left(H_{2}-1\right)} X \Rightarrow H\left(e^{j \omega}\right)=\frac{Y\left(e^{j \omega}\right)}{X\left(e^{j \omega}\right)}=\frac{H_{1}\left(e^{j \omega}\right)}{1+H_{3}\left(e^{j \omega}\right)\left(H_{2}\left(e^{j \omega}\right)-1\right)} \tag{8}
\end{equation*}
$$

PROBLEM 4. Consider the following interconnection of LTI systems:


Express the frequency response of the overall system $H\left(e^{j \omega}\right)$ in terms of the frequency responses of the subsystems depicted in the diagram.

## SOLUTION:

The first thing that we do is to transform all variables to the DTFT domain (we omit the $e^{j \omega}$ terms), to introduce intermediate variables in every connection between system elements and to simplify as much as possible the diagram:


We can observe that there is a feedback loop involving the first addition operator and systems $H_{3}$ and $H_{5}$ (surrounded by a dashed line in the diagram above). The best way to proceed is to first compute the frequency response of the sub-system bounded by the dashed line, i.e. to find the relationship between $D$ and $X$. We can see that the feedback sub-system contains 4 unknowns $(X, E, D, C)$ which means that we will need to write 3 equations:

$$
\begin{align*}
D & =H_{3} E  \tag{9}\\
C & =H_{5} D  \tag{10}\\
E & =X+C \tag{11}
\end{align*}
$$

Combining these three equations:

$$
D=H_{3} X+H_{3} C=H_{3} X+H_{3} H_{5} D \Rightarrow D=\frac{H_{3}}{1-H_{3} H_{5}} X
$$

Then we can also find the relationship between $E$ and the input $X$ :

$$
D=H_{3} E \Rightarrow E=\frac{D}{H_{3}}=\frac{1}{1-H_{3} H_{5}} X
$$

Now we can proceed to determine the overall frequency response of the whole system. Since in the whole system we have 7 unknowns, we need 6 equations to fully determine the output with respect to the input. We already wrote 3 equations above so we just need 3 more:

$$
\begin{align*}
Y & =A+B  \tag{12}\\
A & =H_{1} H_{2} E  \tag{13}\\
B & =H_{4} D \tag{14}
\end{align*}
$$

Combining the three equations above:

$$
Y=A+B=H_{1} H_{2} E+H_{4} D
$$

and using the expressions that we found for $E$ and $D$ with respect to $X$ :

$$
Y=H_{1} H_{2} E+H_{4} D=\frac{H_{1} H_{2}+H_{4} H_{3}}{1-H_{3} H_{5}} X
$$

PROBLEM 5. Consider the interconnection of linear shift-invariant systems in the figure below:

(a) Express the frequency response of the overall system $H\left(e^{j \omega}\right)$ in terms of the frequency responses of the subsystems $H_{1}\left(e^{j \omega}\right), H_{2}\left(e^{j \omega}\right)$ and $H_{3}\left(e^{j \omega}\right)$.
(b) Determine the frequency response $H\left(e^{j \omega}\right)$ of the overall system if:

$$
\begin{aligned}
h_{1}[n] & =\frac{\sin \left(\frac{\pi}{3} n\right)}{\pi n} \\
h_{2}[n] & =(0.3)^{n} \mu[n] \\
h_{3}[n] & =\delta[n-2]
\end{aligned}
$$

## SOLUTION:

The overall frequency response is:

$$
Y=\frac{H_{1} H_{2}}{1-H_{2} H_{3}} X \Rightarrow H=\frac{H_{1} H_{2}}{1-H_{2} H_{3}}
$$

Transforming $h_{1}[n], h_{2}[n], h_{3}[n]$ to the DTFT domain we finally obtain that:

$$
H\left(e^{j \omega}\right)= \begin{cases}\frac{1}{1-0.3 e^{-j \omega}-e^{-j \omega 2}} & |\omega| \leq \omega_{c} \\ 0 & |\omega|>\omega_{c}\end{cases}
$$

PROBLEM 6 (problem 3.59 from the book): An LTI IIR discrete-time system is described by the difference equation

$$
y[n]+a_{1} y[n-1]=b_{0} x[n]+b_{1} x[n-1]
$$

where the input is $x[n]$, the output is $y[n]$, and the constants $a_{1}, b_{0}$ and $b_{1}$ are real. Determine the expression for its frequency response. For what values of $b_{0}$ and $b_{1}$ will the magnitude response be a constant for all values of $\omega$ ?

SOLUTION: In order to obtain the frequency response of the system, first we need to transform the system's equation into the frequency domain:

$$
Y\left(e^{j \omega}\right)+a_{1} e^{-j \omega} Y\left(e^{j \omega}\right)=b_{0} X\left(e^{j \omega}\right)+b_{1} e^{-j \omega} X\left(e^{j \omega}\right)
$$

so the frequency response of the system is:

$$
H\left(e^{j \omega}\right)=\frac{Y\left(e^{j \omega}\right)}{X\left(e^{j \omega}\right)}=\frac{b_{0}+b_{1} e^{-j \omega}}{1+a_{1} e^{-j \omega}}
$$

It is difficult to operate with the requirement $\left|H\left(e^{j \omega}\right)\right|=K=$ constant due to the presence of complex quantities inside the absolute value operator. In order to get rid of complex terms the easiest is to solve for the equivalent requirement $\left.\mid H\left(e^{j \omega}\right)\right)\left.\right|^{2}=$ $K^{2}=$ constant:

$$
\begin{aligned}
\left|H\left(e^{j \omega}\right)\right|^{2} & =H\left(e^{j \omega}\right) H^{*}\left(e^{j \omega}\right)=\frac{\left(b_{0}+b_{1} e^{-j \omega}\right)\left(b_{0}+b_{1} e^{j \omega}\right)}{\left(1+a_{1} e^{-j \omega}\right)\left(1+a_{1} e^{j \omega}\right)} \\
& =\frac{b_{0}^{2}+b_{1}^{2}+b_{0} b_{1}\left(e^{j \omega}+e^{-j \omega}\right)}{1+a_{1}^{2}+a_{1}\left(e^{j \omega}+e^{j \omega}\right)}=\frac{b_{0}^{2}+b_{1}^{2}+2 b_{0} b_{1} \cos \omega}{1+a_{1}^{2}+2 a_{1} \cos \omega}=K^{2}=C
\end{aligned}
$$

Then we have to find the values of $a_{1}, b_{0}$ and $b_{1}$ satifying:

$$
\underbrace{b_{0}^{2}+b_{1}^{2}}_{A}+\underbrace{2 b_{0} b_{1}}_{B} \cos \omega=\underbrace{C+C a_{1}^{2}}_{A^{\prime}}+\underbrace{2 C a_{1}}_{B^{\prime}} \cos \omega
$$

We can see that the expressions at each side of the equation above corresponds to a scaled sinusoid with non-zero mean. So we can enforce the equality by simply enforcing that the mean of the sinusoids is the same $\left(A=A^{\prime}\right)$ and that the scale of both sinusoids is also the same $\left(B=B^{\prime}\right)$ :

$$
\begin{aligned}
& A=A^{\prime} \quad \Rightarrow b_{0}^{2}+b_{1}^{2}=C+C a_{1}^{2} \\
& B=B^{\prime} \Rightarrow b_{0} b_{1}=C a_{1}
\end{aligned}
$$

Putting both equations together:

$$
b_{0}=C \frac{a_{1}}{b_{1}} \Rightarrow \frac{C^{2} a_{1}^{2}}{b_{1}^{2}}+b_{1}^{2}=C+C a_{1}^{2} \Rightarrow b_{1}^{4}-C\left(1+a_{1}^{2}\right) b_{1}^{2}+C^{2} a_{1}^{2}=0
$$

The quadratic equation above has two solutions:

$$
b_{1}^{2}=\frac{C\left(1+a_{1}^{2}\right) \pm \sqrt{C^{2}\left(1+a_{1}^{2}\right)^{2}-4 C^{2} a_{1}^{2}}}{2}
$$

Operating we get that the solution is either $b_{1}= \pm K$ or $b_{1}= \pm K a_{1}$. We first try the former solution to check if it fulfills our requirement:

$$
\left|H\left(e^{j \omega}\right)\right|=\left|\frac{ \pm K a_{1} \pm K e^{-j \omega}}{1+a_{1} e^{-j \omega}}\right|=K\left|\frac{a_{1}+e^{-j \omega}}{1+a_{1} e^{-j \omega}}\right|
$$

Clearly, the expression above is not equal to a constant in general so this is not a valid solution of the problem. We try now the solution $b_{1}= \pm K a_{1}$ :

$$
\left|H\left(e^{j \omega}\right)\right|=\left|\frac{ \pm K \pm K a_{1} e^{-j \omega}}{1+a_{1} e^{-j \omega}}\right|=K\left|\frac{1+a_{1} e^{-j \omega}}{1+a_{1} e^{-j \omega}}\right|=K
$$

And therefore $b_{1}= \pm K a_{1}$ is the solution that we need. The reason for one of the solutions that we found to be invalid is that we substituted the original requirement $\left|H\left(e^{j \omega}\right)\right|=K$ for the alternative requirement $\left|H\left(e^{j \omega}\right)\right|^{2}=K^{2}$. This had the effect of introducing an spurious solution since the latter equality is fulfilled not only when $\left|H\left(e^{j \omega}\right)\right|=K$ but also when $\left|H\left(e^{j \omega}\right)\right|=-K$. Obviously, the latter solution is not valid.

PROBLEM 7: Consider the system defined by the difference equation

$$
y[n]=a y[n-1]+b x[n]+x[n-1]
$$

where $a$ and $b$ are real, and $|a|<1$. Find the relationship between $a$ and $b$ that must exist if the frequency response is to have a constant magnitude for all $\omega$, that is $\left|H\left(e^{j \omega}\right)\right|=1$.

SOLUTION: In order to obtain the frequency response of the system, first we need to transform the system's equation into the frequency domain:

$$
Y\left(e^{j \omega}\right)=a e^{-j \omega} Y\left(e^{j \omega}\right)+b X\left(e^{j \omega}\right)+e^{-j \omega} X\left(e^{j \omega}\right)
$$

so the frequency response of the system is:

$$
H\left(e^{j \omega}\right)=\frac{Y\left(e^{j \omega}\right)}{X\left(e^{j \omega}\right)}=\frac{b+e^{-j \omega}}{1-a \cdot e^{-j \omega}}
$$

If the equality $\left|H\left(e^{j \omega}\right)\right|=1$ hold then it must also hold the equality $\left|H\left(e^{j \omega}\right)\right|^{2}=1$. Solving this latter equality is easier because the expression on the left side has only real terms inside the absolute value operator. Operating a bit:

$$
\left|H\left(e^{j \omega}\right)\right|^{2}=1 \Longrightarrow H\left(e^{j \omega}\right) \cdot H^{*}\left(e^{j \omega}\right)=1
$$

substituting the value of $H\left(e^{j \omega}\right)$ into the expression above we obtain:

$$
H\left(e^{j \omega}\right) \cdot H^{*}\left(e^{j \omega}\right)=\frac{\left(b+e^{-j \omega}\right) \cdot\left(b+e^{j \omega}\right)}{\left(1-a \cdot e^{-j \omega}\right) \cdot\left(1-a \cdot e^{j \omega}\right)}=\frac{1+b^{2}+b \cdot\left(e^{j \omega}+e^{-j \omega}\right)}{1+a^{2}-a \cdot\left(e^{j \omega}+e^{-j \omega}\right)}=1
$$

So, the numerator and denominator of the fraction above must be equal, which translates into the two equations:

$$
\begin{array}{ll}
1+b^{2} & =1+a^{2} \\
b & =-a
\end{array}
$$

Clearly, if and only if $b=-a$ the two equations are fullfiled and $\left|H\left(e^{j \omega}\right)\right|^{2}=1$. Since we have only a single solution to the squared version of our original condition we can conclude that this solution has to be also the solution to our original constraint. That is $\left|H\left(e^{j \omega}\right)\right|=1$ if and only if $b=-a$.

